Fixes to make PolyQuantPullRtac build again, including specializing MTypeUnify to only use pmaps. Next we need to clean up the interface so that PolyQuantPullRtac's use of the abstractions is cleaner (e.g. less need for as many at signs and underscores

examples/PolyRewrite/PolyQuantPullRtac.v
@@ -280,37 +280,26 @@ Arguments Build_Proper_concl {_ _ _} _ _.
 Require Import MirrorCore.Lambda.Polymorphic.
 Require Import MirrorCore.Util.Forwardy.
 
-Print PPr.
-Check do_prespectful.
-
-(* TODO: need to figure out what arguments to fill in here. *)
-Check do_prespectful.
-Check do_respectful.
-SearchAbout mtyp.
-Print do_respectful.
-Print do_prespectful.
-
-Typeclasses eauto := debug.
-
-Locate MTypeUnify.
-
-
-(* force implementation to be pmaps? (in MTypeUnify - maybe?)
+(* force implementation to be pmaps? (in MTypeUnify - maybe?) (done)
    write a convencience wrapper that handles everything for mtyp
    figure out what arguments i want to_respectful/do_prespectful to have
    and then make it have them
-   *)
+ *)
+
+Check do_prespectful.
+
+SearchAbout (positive -> mtyp _).
 
 Definition get_respectful_only_all_ex : respectful_dec typ func Rbase :=
-  do_prespectful (expr_eq_dec _ _) (MTypeUnify.mtype_unify _ _ HintDbs.view_update) _
-  (@PPr _ _ _ 1 (fun T => {|term := Inj (Ex T); relation := Rrespects (Rpointwise T flip_impl) flip_impl |}) ::
-       @PPr _ _ _ 1 (fun T => {|term := Inj (All T); relation := Rrespects (Rpointwise T flip_impl) flip_impl |}) ::
+  do_prespectful rel_dec (MTypeUnify.mtype_unify _) (@tyVar typ')
+                 (@PPr _ _ _ 1 (fun T => {|term := Inj (Ex T); relation := Rrespects (Rpointwise T flip_impl) flip_impl |}) ::
+                       @PPr _ _ _ 1 (fun T => {|term := Inj (All T); relation := Rrespects (Rpointwise T flip_impl) flip_impl |}) ::
      nil).
 
 Definition get_respectful : respectful_dec typ func Rbase :=
-  do_prespectful
-    (PPr 1 (fun T => {|term := Inj (Ex T); relation := Rrespects (Rpointwise T flip_impl) flip_impl |}) ::
-         PPr 1 (fun T => {|term := Inj (All T); relation := Rrespects (Rpointwise T flip_impl) flip_impl |}) ::
+  do_prespectful rel_dec (MTypeUnify.mtype_unify _) (@tyVar typ')
+    (@PPr _ _ _ 1 (fun T => {|term := Inj (Ex T); relation := Rrespects (Rpointwise T flip_impl) flip_impl |}) ::
+         @PPr _ _ _ 1 (fun T => {|term := Inj (All T); relation := Rrespects (Rpointwise T flip_impl) flip_impl |}) ::
          Pr {| term := Inj And; relation := Rrespects flip_impl (Rrespects flip_impl flip_impl) |} ::
          Pr {| term := Inj Or; relation := Rrespects flip_impl (Rrespects flip_impl flip_impl) |} ::
          Pr {| term := Inj Plus;
@@ -332,13 +321,13 @@ Ltac prove_prespectful :=
 Theorem get_respectful_only_all_ex_sound
 : respectful_spec RbaseD get_respectful_only_all_ex.
 Proof.
-  eapply do_prespectful_sound.
-  repeat first [ eapply Forall_cons | eapply Forall_nil ]; simpl; prove_prespectful.
+  eapply do_prespectful_sound; [eapply rel_dec_correct|].
+  repeat first [ eapply Forall_cons | eapply Forall_nil]; simpl; prove_prespectful.
 Qed.
 
 Theorem get_respectful_sound : respectful_spec RbaseD get_respectful.
 Proof.
-  eapply do_prespectful_sound.
+  eapply do_prespectful_sound; [eapply rel_dec_correct|].
   repeat first [eapply Forall_cons | eapply Forall_nil]; prove_prespectful.
 Qed.
 
@@ -413,8 +402,10 @@ Proof.
   { eauto. }
 Qed.
 
+Check RewriteHintDbOk.
+
 Theorem the_rewrites_sound
-: forall hints, RewriteHintDb_sound hints ->
+: forall hints, RewriteHintDbOk RbaseD hints ->
     setoid_rewrite_spec RbaseD (the_rewrites hints).
 Proof.
   unfold the_rewrites. intros.
@@ -433,19 +424,19 @@ Qed.
 
 Definition the_lemmas
   : RewriteHintDb Rbase :=
-  PRw _ 1 lem_pull_ex_and_left IDTACK ::
-     PRw _ 1 lem_pull_ex_and_right IDTACK ::
+  @PRw _ _ _ 1 lem_pull_ex_and_left IDTACK ::
+     @PRw _ _ _ 1 lem_pull_ex_and_right IDTACK ::
      nil.
 
 (* check Polymorphic.v or PolyInst.v  - move the stuff into there. *)
 
 (* need a more convenient interface than raw vectors *)
 (* go from poly n to the actual thing with quantifiers as actual quantifiers *)
-Theorem the_lemmas_sound : RewriteHintDb_sound the_lemmas.
+Theorem the_lemmas_sound : RewriteHintDbOk RbaseD the_lemmas.
 Proof.
   repeat first [ apply Forall_cons | apply Forall_nil ]; split; try apply IDTACK_sound.
-  { intros. unfold Polymorphic.inst. apply lem_pull_ex_and_left_sound. }
-  { intros. unfold Polymorphic.inst. apply lem_pull_ex_and_right_sound. }
+  { unfold polymorphicD. intros. apply lem_pull_ex_and_left_sound. }
+  { unfold polymorphicD. intros. apply lem_pull_ex_and_right_sound. }
 Qed.
 
 Definition pull_all_quant : lem_rewriter typ func Rbase :=
